Add iresult as the 'bubble' semantics

shift-reset/interpreter/interpreter.v
@@ -5,6 +5,11 @@ From shift_reset.interpreter Require Import ierror iheap imonad.
 Local Open Scope string_scope.
 Local Open Scope Z_scope.
 
+Inductive iresult : Type :=
+| RReturn : val -> iresult
+| RBubbleS : (val -> imonad iresult) -> kont2S -> iresult
+| RBubbleC : (val -> imonad iresult) -> kont2C -> iresult.
+
 Definition interpret_atom (a : atom) : imonad val :=
   match a with
   | AUnit => imonad_pure VUnit
@@ -23,28 +28,28 @@ Definition interpret_fun (t : term1) : imonad val :=
 Definition interpret_fix (t : term2) : imonad val :=
   imonad_map (fun env => VFix (C2 env t)) imonad_ask_env.
 
-Definition unwrap_VInt_then (m : imonad val) (k : Z -> imonad val) : imonad val :=
+Definition unwrap_VInt_then {A} (m : imonad val) (k : Z -> imonad A) : imonad A :=
   imonad_bind m
     (fun v => match v with
               | VInt i => k i
               | _ => imonad_throw (TypeError "")
               end).
 
-Definition unwrap_VBool_then (m : imonad val) (k : bool -> imonad val) : imonad val :=
+Definition unwrap_VBool_then {A} (m : imonad val) (k : bool -> imonad A) : imonad A :=
   imonad_bind m
     (fun v => match v with
               | VBool b => k b
               | _ => imonad_throw (TypeError "")
               end).
 
-Definition unwrap_VLoc_then (m : imonad val) (k : loc -> imonad val) : imonad val :=
+Definition unwrap_VLoc_then {A} (m : imonad val) (k : loc -> imonad A) : imonad A :=
   imonad_bind m
     (fun v => match v with
               | VLoc l => k l
               | _ => imonad_throw (TypeError "")
               end).
 
-Definition interpret_if (a : atom) (m1 m2 : imonad val) : imonad val :=
+Definition interpret_if (a : atom) (m1 m2 : imonad iresult) : imonad iresult :=
   unwrap_VBool_then (interpret_atom a) (fun b => if b then m1 else m2).
 
 Definition interpret_i2i (f : Z -> Z) (m : imonad val) : imonad val :=
@@ -92,7 +97,7 @@ Definition interpret_prim2 (p : prim2) (a1 a2 : atom) : imonad val :=
 Definition interpret_pair (a1 a2 : atom) : imonad val :=
   imonad_lift2 VPair (interpret_atom a1) (interpret_atom a2).
 
-Definition interpret_split (a : atom) (k : val -> val -> imonad val) : imonad val :=
+Definition interpret_split (a : atom) (k : val -> val -> imonad iresult) : imonad iresult :=
   imonad_bind (interpret_atom a)
     (fun v => match v with
               | VPair v1 v2 => k v1 v2
@@ -105,7 +110,7 @@ Definition interpret_inl (a : atom) : imonad val :=
 Definition interpret_inr (a : atom) : imonad val :=
   imonad_map VInr (interpret_atom a).
 
-Definition interpret_case (a : atom) (k1 k2 : val -> imonad val) : imonad val :=
+Definition interpret_case (a : atom) (k1 k2 : val -> imonad iresult) : imonad iresult :=
   imonad_bind (interpret_atom a)
     (fun v => match v with
               | VInl v' => k1 v'
@@ -148,167 +153,160 @@ Definition interpret_free (a : atom) : imonad val :=
                           | Some h' => imonad_then (imonad_set_heap h') (imonad_pure VUnit)
                           end)).
 
-Definition with_binder (b : binder) (v : val) (m : imonad val) : imonad val :=
+Definition with_binder (b : binder) (v : val) (m : imonad iresult) : imonad iresult :=
   match b with
   | BAnon => m
   | BVar x => imonad_local_env (ECons x v) m
   end.
 
-Definition interpret_term1_with (rec : term -> imonad val) (t : term1) (v : val) : imonad val :=
+Definition interpret_term1_with (rec : term -> imonad iresult) (t : term1) (v : val) : imonad iresult :=
   let (b, t') := t in with_binder b v (rec t').
 
-Definition interpret_term2_with (rec : term -> imonad val) (t : term2) (v1 v2 : val) : imonad val :=
+Definition interpret_term2_with (rec : term -> imonad iresult) (t : term2) (v1 v2 : val) : imonad iresult :=
   let (b1, b2, t') := t in with_binder b1 v1 (with_binder b2 v2 (rec t')).
 
-Definition interpret_clo1_with (rec : term -> imonad val) (c : clo1) (m : imonad val) : imonad val :=
+Definition interpret_clo1_with (rec : term -> imonad iresult) (c : clo1) (m : imonad val) : imonad iresult :=
   imonad_bind m (fun v => let (env, t) := c in imonad_local_env (fun _ => env) (interpret_term1_with rec t v)).
 
-Definition interpret_clo2_with (rec : term -> imonad val) (c : clo2) (f : val) (m : imonad val) : imonad val :=
+Definition interpret_clo2_with (rec : term -> imonad iresult) (c : clo2) (f : val) (m : imonad val) : imonad iresult :=
   imonad_bind m (fun v => let (env, t) := c in imonad_local_env (fun _ => env) (interpret_term2_with rec t f v)).
 
+(*
 Definition interpret_kont_with (rec : kont -> term -> imonad val) (k : kont) (m : imonad val) : imonad val :=
   match k with
   | KNil => m
   | KCons c k' => interpret_clo1_with (rec k') c m
   end.
-
-Inductive delim : Type :=
-| DNone : delim
-| DReset : delim
-| DPrompt : delim.
+*)
 
 Set Implicit Arguments.
 
-Inductive term_graph : delim -> kont -> term -> Prop :=
-| GTAtom d k a : kont_graph d k -> term_graph d k (TAtom a)
-| GTFun d k t' : kont_graph d k -> term_graph d k (TFun t')
-| GTFix d k t' : kont_graph d k -> term_graph d k (TFix t')
-| GTApp d k a1 a2 : kont_graph d k -> term_graph d k (TApp a1 a2)
-| GTLet d k t1 t2 : (forall env, term_graph d (KCons (C1 env t2) k) t1) -> term_graph d k (TLet t1 t2)
-| GTIf d k a t1 t2 : term_graph d k t1 -> term_graph d k t2 -> term_graph d k (TIf a t1 t2)
-| GTPrim1 d k p a : kont_graph d k -> term_graph d k (TPrim1 p a)
-| GTPrim2 d k p a1 a2 : kont_graph d k -> term_graph d k (TPrim2 p a1 a2)
-| GTPair d k a1 a2 : kont_graph d k -> term_graph d k (TPair a1 a2)
-| GTSplit d k a t' : term2_graph d k t' -> term_graph d k (TSplit a t')
-| GTInl d k a : kont_graph d k -> term_graph d k (TInl a)
-| GTInr d k a : kont_graph d k -> term_graph d k (TInr a)
-| GTCase d k a t1 t2 : term1_graph d k t1 -> term1_graph d k t2 -> term_graph d k (TCase a t1 t2)
-| GTRef d k a : kont_graph d k -> term_graph d k (TRef a)
-| GTGet d k a : kont_graph d k -> term_graph d k (TGet a)
-| GTSet d k a1 a2 : kont_graph d k -> term_graph d k (TSet a1 a2)
-| GTFree d k a : kont_graph d k -> term_graph d k (TFree a)
-| GTShiftX k t' : term_graph DNone k (TShift t')
-| GTShiftS k t' : term1_graph DReset KNil t' -> term_graph DReset k (TShift t')
-| GTShiftC k t' : term_graph DPrompt k (TShift t')
-| GTReset d k t' : term_graph DReset KNil t' -> kont_graph d k -> term_graph d k (TReset t')
-| GTControlX k t' : term_graph DNone k (TControl t')
-| GTControlS k t' : term_graph DReset k (TControl t')
-| GTControlC k t' : term1_graph DPrompt KNil t' -> term_graph DPrompt k (TControl t')
-| GTPrompt d k t' : term_graph DPrompt KNil t' -> kont_graph d k -> term_graph d k (TPrompt t')
-with term1_graph : delim -> kont -> term1 -> Prop :=
-| GT1 d k b t' : term_graph d k t' -> term1_graph d k (T1 b t')
-with term2_graph : delim -> kont -> term2 -> Prop :=
-| GT2 d k b1 b2 t' : term_graph d k t' -> term2_graph d k (T2 b1 b2 t')
-with clo1_graph : delim -> kont -> clo1 -> Prop :=
-| GC1 d k env t : term1_graph d k t -> clo1_graph d k (C1 env t)
-with kont_graph : delim -> kont -> Prop :=
-| GKNil d : kont_graph d KNil
-| GKCons d c k' : clo1_graph d k' c -> kont_graph d (KCons c k').
+Inductive term_graph : kont1 -> term -> Prop :=
+| GTAtom k a : kont1_graph k -> term_graph k (TAtom a)
+| GTFun k t' : kont1_graph k -> term_graph k (TFun t')
+| GTFix k t' : kont1_graph k -> term_graph k (TFix t')
+| GTApp k a1 a2 : kont1_graph k -> term_graph k (TApp a1 a2)
+| GTLet k t1 t2 : (forall env, term_graph (K1Cons (C1 env t2) k) t1) -> term_graph k (TLet t1 t2)
+| GTIf k a t1 t2 : term_graph k t1 -> term_graph k t2 -> term_graph k (TIf a t1 t2)
+| GTPrim1 k p a : kont1_graph k -> term_graph k (TPrim1 p a)
+| GTPrim2 k p a1 a2 : kont1_graph k -> term_graph k (TPrim2 p a1 a2)
+| GTPair k a1 a2 : kont1_graph k -> term_graph k (TPair a1 a2)
+| GTSplit k a t' : term2_graph k t' -> term_graph k (TSplit a t')
+| GTInl k a : kont1_graph k -> term_graph k (TInl a)
+| GTInr k a : kont1_graph k -> term_graph k (TInr a)
+| GTCase k a t1 t2 : term1_graph k t1 -> term1_graph k t2 -> term_graph k (TCase a t1 t2)
+| GTRef k a : kont1_graph k -> term_graph k (TRef a)
+| GTGet k a : kont1_graph k -> term_graph k (TGet a)
+| GTSet k a1 a2 : kont1_graph k -> term_graph k (TSet a1 a2)
+| GTFree k a : kont1_graph k -> term_graph k (TFree a)
+| GTShift k t' : term1_graph K1Nil t' -> term_graph k (TShift t')
+| GTReset k t' : term_graph K1Nil t' -> kont1_graph k -> term_graph k (TReset t')
+| GTControl k t' : term1_graph K1Nil t' -> term_graph k (TControl t')
+| GTPrompt k t' : term_graph K1Nil t' -> kont1_graph k -> term_graph k (TPrompt t')
+with term1_graph : kont1 -> term1 -> Prop :=
+| GT1 k b t' : term_graph k t' -> term1_graph k (T1 b t')
+with term2_graph : kont1 -> term2 -> Prop :=
+| GT2 k b1 b2 t' : term_graph k t' -> term2_graph k (T2 b1 b2 t')
+with clo1_graph : kont1 -> clo1 -> Prop :=
+| GC1 k env t : term1_graph k t -> clo1_graph k (C1 env t)
+with kont1_graph : kont1 -> Prop :=
+| GK1Nil : kont1_graph K1Nil
+| GK1Cons c k' : clo1_graph k' c -> kont1_graph (K1Cons c k').
 
-Lemma GTAtom_inv d k a : term_graph d k (TAtom a) -> kont_graph d k.
+Lemma GTAtom_inv k a : term_graph k (TAtom a) -> kont1_graph k.
 Proof. inversion 1; auto. Defined.
 
-Lemma GTFun_inv d k t' : term_graph d k (TFun t') -> kont_graph d k.
+Lemma GTFun_inv k t' : term_graph k (TFun t') -> kont1_graph k.
 Proof. inversion 1; auto. Defined.
 
-Lemma GTFix_inv d k t' : term_graph d k (TFix t') -> kont_graph d k.
+Lemma GTFix_inv k t' : term_graph k (TFix t') -> kont1_graph k.
 Proof. inversion 1; auto. Defined.
 
-Lemma GTApp_inv d k a1 a2 : term_graph d k (TApp a1 a2) -> kont_graph d k.
+Lemma GTApp_inv k a1 a2 : term_graph k (TApp a1 a2) -> kont1_graph k.
 Proof. inversion 1; auto. Defined.
 
-Lemma GTLet_inv d k t1 t2 : term_graph d k (TLet t1 t2) -> forall env, term_graph d (KCons (C1 env t2) k) t1.
+Lemma GTLet_inv k t1 t2 : term_graph k (TLet t1 t2) -> forall env, term_graph (K1Cons (C1 env t2) k) t1.
 Proof. inversion 1; auto. Defined.
 
-Lemma GTIf_inv1 d k a t1 t2 : term_graph d k (TIf a t1 t2) -> term_graph d k t1.
+Lemma GTIf_inv1 k a t1 t2 : term_graph k (TIf a t1 t2) -> term_graph k t1.
 Proof. inversion 1; auto. Defined.
 
-Lemma GTIf_inv2 d k a t1 t2 : term_graph d k (TIf a t1 t2) -> term_graph d k t2.
+Lemma GTIf_inv2 k a t1 t2 : term_graph k (TIf a t1 t2) -> term_graph k t2.
 Proof. inversion 1; auto. Defined.
 
-Lemma GTPrim1_inv d k p a : term_graph d k (TPrim1 p a) -> kont_graph d k.
+Lemma GTPrim1_inv k p a : term_graph k (TPrim1 p a) -> kont1_graph k.
 Proof. inversion 1; auto. Defined.
 
-Lemma GTPrim2_inv d k p a1 a2 : term_graph d k (TPrim2 p a1 a2) -> kont_graph d k.
+Lemma GTPrim2_inv k p a1 a2 : term_graph k (TPrim2 p a1 a2) -> kont1_graph k.
 Proof. inversion 1; auto. Defined.
 
-Lemma GTPair_inv d k a1 a2 : term_graph d k (TPair a1 a2) -> kont_graph d k.
+Lemma GTPair_inv k a1 a2 : term_graph k (TPair a1 a2) -> kont1_graph k.
 Proof. inversion 1; auto. Defined.
 
-Lemma GTSplit_inv d k a t' : term_graph d k (TSplit a t') -> term2_graph d k t'.
+Lemma GTSplit_inv k a t' : term_graph k (TSplit a t') -> term2_graph k t'.
 Proof. inversion 1; auto. Defined.
 
-Lemma GTInl_inv d k a : term_graph d k (TInl a) -> kont_graph d k.
+Lemma GTInl_inv k a : term_graph k (TInl a) -> kont1_graph k.
 Proof. inversion 1; auto. Defined.
 
-Lemma GTInr_inv d k a : term_graph d k (TInr a) -> kont_graph d k.
+Lemma GTInr_inv k a : term_graph k (TInr a) -> kont1_graph k.
 Proof. inversion 1; auto. Defined.
 
-Lemma GTCase_inv1 d k a t1 t2 : term_graph d k (TCase a t1 t2) -> term1_graph d k t1.
+Lemma GTCase_inv1 k a t1 t2 : term_graph k (TCase a t1 t2) -> term1_graph k t1.
 Proof. inversion 1; auto. Defined.
 
-Lemma GTCase_inv2 d k a t1 t2 : term_graph d k (TCase a t1 t2) -> term1_graph d k t2.
+Lemma GTCase_inv2 k a t1 t2 : term_graph k (TCase a t1 t2) -> term1_graph k t2.
 Proof. inversion 1; auto. Defined.
 
-Lemma GTRef_inv d k a : term_graph d k (TRef a) -> kont_graph d k.
+Lemma GTRef_inv k a : term_graph k (TRef a) -> kont1_graph k.
 Proof. inversion 1; auto. Defined.
 
-Lemma GTGet_inv d k a : term_graph d k (TGet a) -> kont_graph d k.
+Lemma GTGet_inv k a : term_graph k (TGet a) -> kont1_graph k.
 Proof. inversion 1; auto. Defined.
 
-Lemma GTSet_inv d k a1 a2 : term_graph d k (TSet a1 a2) -> kont_graph d k.
+Lemma GTSet_inv k a1 a2 : term_graph k (TSet a1 a2) -> kont1_graph k.
 Proof. inversion 1; auto. Defined.
 
-Lemma GTFree_inv d k a : term_graph d k (TFree a) -> kont_graph d k.
+Lemma GTFree_inv k a : term_graph k (TFree a) -> kont1_graph k.
 Proof. inversion 1; auto. Defined.
 
-Lemma GTShiftS_inv k t' : term_graph DReset k (TShift t') -> term1_graph DReset KNil t'.
+Lemma GTShift_inv k t' : term_graph k (TShift t') -> term1_graph K1Nil t'.
 Proof. inversion 1; auto. Defined.
 
-Lemma GTReset_inv1 d k t' : term_graph d k (TReset t') -> term_graph DReset KNil t'.
+Lemma GTReset_inv1 k t' : term_graph k (TReset t') -> term_graph K1Nil t'.
 Proof. inversion 1; auto. Defined.
 
-Lemma GTReset_inv2 d k t' : term_graph d k (TReset t') -> kont_graph d k.
+Lemma GTReset_inv2 k t' : term_graph k (TReset t') -> kont1_graph k.
 Proof. inversion 1; auto. Defined.
 
-Lemma GTControlC_inv k t' : term_graph DPrompt k (TControl t') -> term1_graph DPrompt KNil t'.
+Lemma GTControl_inv k t' : term_graph k (TControl t') -> term1_graph K1Nil t'.
 Proof. inversion 1; auto. Defined.
 
-Lemma GTPrompt_inv1 d k t' : term_graph d k (TPrompt t') -> term_graph DPrompt KNil t'.
+Lemma GTPrompt_inv1 k t' : term_graph k (TPrompt t') -> term_graph K1Nil t'.
 Proof. inversion 1; auto. Defined.
 
-Lemma GTPrompt_inv2 d k t' : term_graph d k (TPrompt t') -> kont_graph d k.
+Lemma GTPrompt_inv2 k t' : term_graph k (TPrompt t') -> kont1_graph k.
 Proof. inversion 1; auto. Defined.
 
-Lemma GT1_inv d k b t' : term1_graph d k (T1 b t') -> term_graph d k t'.
+Lemma GT1_inv k b t' : term1_graph k (T1 b t') -> term_graph k t'.
 Proof. inversion 1; auto. Defined.
 
-Lemma GT2_inv d k b1 b2 t' : term2_graph d k (T2 b1 b2 t') -> term_graph d k t'.
+Lemma GT2_inv k b1 b2 t' : term2_graph k (T2 b1 b2 t') -> term_graph k t'.
 Proof. inversion 1; auto. Defined.
 
-Lemma GC1_inv d k env t : clo1_graph d k (C1 env t) -> term1_graph d k t.
+Lemma GC1_inv k env t : clo1_graph k (C1 env t) -> term1_graph k t.
 Proof. inversion 1; auto. Defined.
 
-Lemma GKCons_inv d c k' : kont_graph d (KCons c k') -> clo1_graph d k' c.
+Lemma GK1Cons_inv c k' : kont1_graph (K1Cons c k') -> clo1_graph k' c.
 Proof. inversion 1; auto. Defined.
 
-Fixpoint build_term_graph_dep d k (G : kont_graph d k) t : term_graph d k t :=
+Fixpoint build_term_graph_dep (k : kont1) (G : kont1_graph k) (t : term) : term_graph k t :=
   match t with
   | TAtom a => GTAtom a G
   | TFun t' => GTFun t' G
   | TFix t' => GTFix t' G
   | TApp a1 a2 => GTApp a1 a2 G
-  | TLet t1 t2 => GTLet (fun env => build_term_graph_dep (GKCons (GC1 env (build_term1_graph_dep G t2))) t1)
+  | TLet t1 t2 => GTLet (fun env => build_term_graph_dep (GK1Cons (GC1 env (build_term1_graph_dep G t2))) t1)
   | TIf a t1 t2 => GTIf a (build_term_graph_dep G t1) (build_term_graph_dep G t2)
   | TPrim1 p a => GTPrim1 p a G
   | TPrim2 p a1 a2 => GTPrim2 p a1 a2 G
@@ -321,109 +319,105 @@ Fixpoint build_term_graph_dep d k (G : kont_graph d k) t : term_graph d k t :=
   | TGet a => GTGet a G
   | TSet a1 a2 => GTSet a1 a2 G
   | TFree a => GTFree a G
-  | TShift t' =>
-      match d with
-      | DNone => GTShiftX k t'
-      | DReset => GTShiftS k (build_term1_graph_dep (GKNil DReset) t')
-      | DPrompt => GTShiftC k t'
-      end
-  | TReset t' => GTReset (build_term_graph_dep (GKNil DReset) t') G
-  | TControl t' =>
-      match d with
-      | DNone => GTControlX k t'
-      | DReset => GTControlS k t'
-      | DPrompt => GTControlC k (build_term1_graph_dep (GKNil DPrompt) t')
-      end
-  | TPrompt t' => GTPrompt (build_term_graph_dep (GKNil DPrompt) t') G
+  | TShift t' => GTShift k (build_term1_graph_dep GK1Nil t')
+  | TReset t' => GTReset (build_term_graph_dep GK1Nil t') G
+  | TControl t' => GTControl k (build_term1_graph_dep GK1Nil t')
+  | TPrompt t' => GTPrompt (build_term_graph_dep GK1Nil t') G
   end
-with build_term1_graph_dep d k (G : kont_graph d k) t : term1_graph d k t :=
+with build_term1_graph_dep (k : kont1) (G : kont1_graph k) (t : term1) : term1_graph k t :=
   match t with
   | T1 b t' => GT1 b (build_term_graph_dep G t')
   end
-with build_term2_graph_dep d k (G : kont_graph d k) t : term2_graph d k t :=
+with build_term2_graph_dep (k : kont1) (G : kont1_graph k) (t : term2) : term2_graph k t :=
   match t with
   | T2 b1 b2 t' => GT2 b1 b2 (build_term_graph_dep G t')
   end.
 
-Definition build_clo1_graph_dep d k (G : kont_graph d k) c : clo1_graph d k c :=
+Definition build_clo1_graph_dep (k : kont1) (G : kont1_graph k) (c : clo1) : clo1_graph k c :=
   match c with
   | C1 env t => GC1 env (build_term1_graph_dep G t)
   end.
 
-Fixpoint interpret_term_dep (rec : delim -> kont -> term -> imonad val) d k t (G : term_graph d k t) : imonad val :=
-  match t return term_graph d k t -> imonad val with
-  | TAtom a => fun G => interpret_kont_dep rec (GTAtom_inv G) (interpret_atom a)
-  | TFun t' => fun G => interpret_kont_dep rec (GTFun_inv G) (interpret_fun t')
-  | TFix t' => fun G => interpret_kont_dep rec (GTFix_inv G) (interpret_fix t')
+Fixpoint interpret_term_dep (rec : kont1 -> term -> imonad iresult) (k : kont1) (t : term) (G : term_graph k t) : imonad iresult :=
+  match t return term_graph k t -> imonad iresult with
+  | TAtom a => fun G => interpret_kont1_dep rec (GTAtom_inv G) (interpret_atom a)
+  | TFun t' => fun G => interpret_kont1_dep rec (GTFun_inv G) (interpret_fun t')
+  | TFix t' => fun G => interpret_kont1_dep rec (GTFix_inv G) (interpret_fix t')
   | TApp a1 a2 =>
       fun G =>
         let m1 := interpret_atom a1 in
         let m2 := interpret_atom a2 in
         imonad_bind m1
           (fun v => match v with
-                    | VFun c => interpret_clo1_with (rec d k) c m2
-                    | VFix c => interpret_clo2_with (rec d k) c v m2
-                    | VKontS k' => interpret_kont_dep rec (GTApp_inv G) (interpret_kont_with (rec DReset) k' m2)
-                    | VKontC k' => interpret_kont_with (rec d) (kont_append k' k) m2
+                    | VFun c => interpret_clo1_with (rec k) c m2
+                    | VFix c => interpret_clo2_with (rec k) c v m2
+                    | VKontS k' => imonad_throw (TypeError "") (*interpret_kont1_dep rec (GTApp_inv G) (interpret_kont_with (rec DReset) k' m2)*)
+                    | VKontC k' => imonad_throw (TypeError "") (*interpret_kont_with (rec d) (kont_append k' k) m2*)
                     | _ => imonad_throw (TypeError "")
                     end)
   | TLet t1 t2 => fun G => imonad_bind imonad_ask_env (fun env => interpret_term_dep rec (GTLet_inv G env))
   | TIf a t1 t2 => fun G => interpret_if a (interpret_term_dep rec (GTIf_inv1 G)) (interpret_term_dep rec (GTIf_inv2 G))
-  | TPrim1 p a => fun G => interpret_kont_dep rec (GTPrim1_inv G) (interpret_prim1 p a)
-  | TPrim2 p a1 a2 => fun G => interpret_kont_dep rec (GTPrim2_inv G) (interpret_prim2 p a1 a2)
-  | TPair a1 a2 => fun G => interpret_kont_dep rec (GTPair_inv G) (interpret_pair a1 a2)
+  | TPrim1 p a => fun G => interpret_kont1_dep rec (GTPrim1_inv G) (interpret_prim1 p a)
+  | TPrim2 p a1 a2 => fun G => interpret_kont1_dep rec (GTPrim2_inv G) (interpret_prim2 p a1 a2)
+  | TPair a1 a2 => fun G => interpret_kont1_dep rec (GTPair_inv G) (interpret_pair a1 a2)
   | TSplit a t' => fun G => interpret_split a (interpret_term2_dep rec (GTSplit_inv G))
-  | TInl a => fun G => interpret_kont_dep rec (GTInl_inv G) (interpret_inl a)
-  | TInr a => fun G => interpret_kont_dep rec (GTInr_inv G) (interpret_inr a)
+  | TInl a => fun G => interpret_kont1_dep rec (GTInl_inv G) (interpret_inl a)
+  | TInr a => fun G => interpret_kont1_dep rec (GTInr_inv G) (interpret_inr a)
   | TCase a t1 t2 => fun G => interpret_case a (interpret_term1_dep rec (GTCase_inv1 G)) (interpret_term1_dep rec (GTCase_inv2 G))
-  | TRef a => fun G => interpret_kont_dep rec (GTRef_inv G) (interpret_ref a)
-  | TGet a => fun G => interpret_kont_dep rec (GTGet_inv G) (interpret_get a)
-  | TSet a1 a2 => fun G => interpret_kont_dep rec (GTSet_inv G) (interpret_set a1 a2)
-  | TFree a => fun G => interpret_kont_dep rec (GTFree_inv G) (interpret_free a)
-  | TShift t' =>
-      match d return term_graph d k (TShift t') -> imonad val with
-      | DNone => fun _ => imonad_throw (ControlError "")
-      | DReset => fun G => interpret_term1_dep rec (GTShiftS_inv G) (VKontS k)
-      | DPrompt => fun _ => imonad_throw (ControlError "")
-      end
-  | TReset t' => fun G => interpret_kont_dep rec (GTReset_inv2 G) (interpret_term_dep rec (GTReset_inv1 G))
-  | TControl t' =>
-      match d return term_graph d k (TControl t') -> imonad val with
-      | DNone => fun _ => imonad_throw (ControlError "")
-      | DReset => fun _ => imonad_throw (ControlError "")
-      | DPrompt => fun G => interpret_term1_dep rec (GTControlC_inv G) (VKontC k)
-      end
-  | TPrompt t' => fun G => interpret_kont_dep rec (GTPrompt_inv2 G) (interpret_term_dep rec (GTPrompt_inv1 G))
+  | TRef a => fun G => interpret_kont1_dep rec (GTRef_inv G) (interpret_ref a)
+  | TGet a => fun G => interpret_kont1_dep rec (GTGet_inv G) (interpret_get a)
+  | TSet a1 a2 => fun G => interpret_kont1_dep rec (GTSet_inv G) (interpret_set a1 a2)
+  | TFree a => fun G => interpret_kont1_dep rec (GTFree_inv G) (interpret_free a)
+  | TShift t' => fun G => imonad_pure (RBubbleS (interpret_term1_dep rec (GTShift_inv G)) (K2SHead k))
+  | TReset t' =>
+      fun G =>
+        imonad_bind (interpret_term_dep rec (GTReset_inv1 G))
+          (fun r =>
+             match r with
+             | RReturn v => interpret_kont1_dep rec (GTReset_inv2 G) (imonad_pure v)
+             | RBubbleS rec' ks => rec' (VKontS ks)
+             | RBubbleC rec' kc => imonad_pure (RBubbleC rec' (K2CSnoc kc k))
+             end)
+  | TControl t' => fun G => imonad_pure (RBubbleC (interpret_term1_dep rec (GTControl_inv G)) (K2CHead k))
+  | TPrompt t' =>
+      fun G =>
+        imonad_bind (interpret_term_dep rec (GTPrompt_inv1 G))
+          (fun r =>
+             match r with
+             | RReturn v => interpret_kont1_dep rec (GTPrompt_inv2 G) (imonad_pure v)
+             | RBubbleS rec' ks => rec' (VKontS ks)
+             | RBubbleC rec' kc => imonad_pure (RBubbleC rec' (K2CSnoc kc k))
+             end)
   end G
-with interpret_term1_dep (rec : delim -> kont -> term -> imonad val) d k t (G : term1_graph d k t) (v : val) : imonad val :=
-  match t return term1_graph d k t -> imonad val with
+with interpret_term1_dep (rec : kont1 -> term -> imonad iresult) (k : kont1) (t : term1) (G : term1_graph k t) (v : val) : imonad iresult :=
+  match t return term1_graph k t -> imonad iresult with
   | T1 b t' => fun G => with_binder b v (interpret_term_dep rec (GT1_inv G))
   end G
-with interpret_term2_dep (rec : delim -> kont -> term -> imonad val) d k t (G : term2_graph d k t) (v1 v2 : val) : imonad val :=
-  match t return term2_graph d k t -> imonad val with
+with interpret_term2_dep (rec : kont1 -> term -> imonad iresult) (k : kont1) (t : term2) (G : term2_graph k t) (v1 v2 : val) : imonad iresult :=
+  match t return term2_graph k t -> imonad iresult with
   | T2 b1 b2 t' => fun G => with_binder b1 v1 (with_binder b2 v2 (interpret_term_dep rec (GT2_inv G)))
   end G
-with interpret_clo1_dep (rec : delim -> kont -> term -> imonad val) d k c (G : clo1_graph d k c) (m : imonad val) : imonad val :=
+with interpret_clo1_dep (rec : kont1 -> term -> imonad iresult) (k : kont1) (c : clo1) (G : clo1_graph k c) (m : imonad val) : imonad iresult :=
   imonad_bind m
-    (fun v => match c return clo1_graph d k c -> imonad val with
+    (fun v => match c return clo1_graph k c -> imonad iresult with
               | C1 env t => fun G => imonad_local_env (fun _ => env) (interpret_term1_dep rec (GC1_inv G) v)
               end G)
-with interpret_kont_dep (rec : delim -> kont -> term -> imonad val) d k (G : kont_graph d k) (m : imonad val) : imonad val :=
-  match k return kont_graph d k -> imonad val with
-  | KNil => fun _ => m
-  | KCons c k' => fun G => interpret_clo1_dep rec (GKCons_inv G) m
+with interpret_kont1_dep (rec : kont1 -> term -> imonad iresult) (k : kont1) (G : kont1_graph k) (m : imonad val) : imonad iresult :=
+  match k return kont1_graph k -> imonad iresult with
+  | K1Nil => fun _ => imonad_map RReturn m
+  | K1Cons c k' => fun G => interpret_clo1_dep rec (GK1Cons_inv G) m
   end G.
 
 Unset Implicit Arguments.
 
-Fixpoint build_kont_graph (d : delim) (k : kont) : kont_graph d k :=
+Fixpoint build_kont1_graph (k : kont1) : kont1_graph k :=
   match k with
-  | KNil => GKNil d
-  | KCons c k' => GKCons (build_clo1_graph_dep (build_kont_graph d k') c)
+  | K1Nil => GK1Nil
+  | K1Cons c k' => GK1Cons (build_clo1_graph_dep (build_kont1_graph k') c)
   end.
 
 Definition build_term_graph (d : delim) (k : kont) (t : term) : term_graph d k t :=
-  build_term_graph_dep (build_kont_graph d k) t.
+  build_term_graph_dep (build_kont1_graph d k) t.
 
 Definition interpret_term_aux (rec : delim -> kont -> term -> imonad val) (d : delim) (k : kont) (t : term) : imonad val :=
   interpret_term_dep rec (build_term_graph d k t).
